Identifier renamings.

Client.ec
@@ -151,14 +151,13 @@ module GReal(Adv : ADV) : GAME = {
   }
 }.
 
-(* Client's Simulator's interface to Ideal Functionality *)
+(* Client's Simulator's interface to Ideal Game *)
 
-module type SIF = {
-  (* ask Ideal Functionality for next query along with its
-     count; None means no more queries
+module type SIG = {
+  (* ask Ideal Game for next query along with its count; None means no
+     more queries
 
-     this involves the Ideal Functionality communicating
-     with Adversary *)
+     this involves the Ideal Game communicating with Adversary *)
 
   proc get_qry_count(cv : client_view) : (elem * int) option
 
@@ -170,11 +169,11 @@ module type SIF = {
 (* module type for Client's Simulator
 
    parameterized by random oracle and Simulator's interface to Ideal
-   Functionality, SIF
+   Game, SIG
 
-   only client_loop may call procedures of SIF *)
+   only client_loop may call procedures of SIG *)
 
-module type SIM(O : RO.OR, SIF : SIF) = {
+module type SIM(O : RO.OR, SIG : SIG) = {
   (* initialization *)
 
   proc * init() : unit
@@ -185,17 +184,15 @@ module type SIM(O : RO.OR, SIF : SIF) = {
 
   (* run the Client's query loop *)
 
-  proc client_loop() : unit {O.hash SIF.get_qry_count SIF.qry_done}
+  proc client_loop() : unit {O.hash SIG.get_qry_count SIG.qry_done}
 }.
 
 (* the "ideal" game
 
    parameterized by Adversary and Simulator for Client
 
-   Server/Client shared secret no longer used
-
-   hashed database is no longer used by Server/TP; instead an
-   elements counts map is used for processing Client queries *)
+   database is turned into elements counts map, which is used for
+   processing Simulator's queries *)
 
 module GIdeal (Adv : ADV, Sim : SIM) : GAME = {
   module Or  = RO.Or        (* random oracle *)
@@ -217,9 +214,9 @@ module GIdeal (Adv : ADV, Sim : SIM) : GAME = {
     }
   }
 
-  (* Simulator's interface to Ideal Functionality *)
+  (* Simulator's interface to Ideal Game *)
 
-  module SIF : SIF = {
+  module SIG : SIG = {
     proc get_qry_count(cv : client_view) : (elem * int) option = {
       var qry_opt : elem option;
       var qry_cnt_opt : (elem * int) option;
@@ -249,8 +246,8 @@ module GIdeal (Adv : ADV, Sim : SIM) : GAME = {
     }
   }
 
-  (* connect Simulator with Or and SIF *)
-  module S = Sim(Or, SIF)
+  (* connect Simulator with Or and SIG *)
+  module S = Sim(Or, SIG)
 
   proc main() : bool = {
     var db_opt : db option; var b : bool; var adv_within_budg : bool;
@@ -280,7 +277,7 @@ module GIdeal (Adv : ADV, Sim : SIM) : GAME = {
 
 (* Client's Simulator *)
 
-module (Sim : SIM) (O : RO.OR, SIF : SIF) = {
+module (Sim : SIM) (O : RO.OR, SIG : SIG) = {
   var cv : client_view
   var sec : sec
 
@@ -298,7 +295,7 @@ module (Sim : SIM) (O : RO.OR, SIF : SIF) = {
     var qry_cnt_opt : (elem * int) option;
     var not_done : bool <- true;
     while (not_done) {
-      qry_cnt_opt <@ SIF.get_qry_count(cv);
+      qry_cnt_opt <@ SIG.get_qry_count(cv);
       if (qry_cnt_opt = None) {
         not_done <- false;
         cv <- cv ++ [cv_got_qry None];
@@ -308,7 +305,7 @@ module (Sim : SIM) (O : RO.OR, SIF : SIF) = {
         cv <- cv ++ [cv_got_qry (Some qry)];
         tag <@ O.hash((qry, sec));
         cv <- cv ++ [cv_query_count(qry, tag, cnt)];
-        SIF.qry_done(cv);
+        SIG.qry_done(cv);
       }
     }
   }
@@ -2918,8 +2915,8 @@ local lemma G7_GIdeal_client_loop :
    ={cv}(G7, Sim)].
 proof.
 proc.
-inline GIdeal(Adv, Sim).SIF.get_qry_count
-       GIdeal(Adv, Sim).SIF.qry_done
+inline GIdeal(Adv, Sim).SIG.get_qry_count
+       GIdeal(Adv, Sim).SIG.qry_done
        G7.tp_count_elem.
 while
   (={not_done} /\ ={glob RO.Or, glob CRO.COr, glob Adv} /\
